Auxiliary/Definitions.dfy
@@ -1,0 +1,47 @@
+
+datatype interview = Null | Node (Key:int, True:interview, False:interview)
+type candidate = map<int, bool>
+
+
+ghost function max(a:nat, b:nat) : nat
+{
+    if a > b then a else b
+}
+
+
+ghost function Depth(iv:interview) : nat
+{
+  if iv == Null then 0 else 1 + max(Depth(iv.True), Depth(iv.False))
+}
+
+ghost function AllKeysIn(iv: interview, S: set<int>): bool
+{
+  match iv
+    case Null => true
+    case Node(k, t, f) =>
+      k in S &&
+      AllKeysIn(t, S) &&
+      AllKeysIn(f, S)
+}
+
+ghost function EveryPathHasCandidate(iv: interview,
+                                     Candidates: set<map<int,bool>>): bool
+{
+  PathMatches(iv, Candidates, map[])
+}
+ghost function PathMatches(iv: interview,
+                          Candidates: set<map<int,bool>>,
+                          prefix: map<int,bool>): bool
+{
+  match iv
+    case Null =>
+      exists c | c in Candidates :: Consistent(c, prefix)
+
+    case Node(k, t, f) =>
+      PathMatches(t, Candidates, prefix[k := true]) &&
+      PathMatches(f, Candidates, prefix[k := false])
+}
+ghost function Consistent(c: map<int,bool>, prefix: map<int,bool>): bool
+{
+  forall k | k in prefix.Keys :: k in c.Keys && c[k] == prefix[k]
+}
