Auxiliary/Interview.dfy
@@ -1,0 +1,41 @@
+include "../Auxiliary/Lemmas.dfy"
+include "../Problems/CDPC.dfy"
+
+
+type Interview< T(==) > {
+
+  ghost function Model():interview
+
+  ghost function Valid():bool
+  {
+    AllKeysIn(Model(), Questions()) &&
+    EveryPathHasCandidate(Model(), Candidates()) &&
+    (forall c1, c2:candidate |  c1 in Candidates() && c2 in Candidates() :: c1.Keys == c2.Keys) &&
+    (forall c:candidate | c in Candidates() :: (c.Keys == Questions()))
+  }
+
+  ghost function Candidates():set<candidate>
+
+  ghost function Questions():set<int>
+
+  ghost function UBSize():nat
+  {
+    |Questions()| * |Candidates()|
+  }
+
+  method {:axiom} Get(b:bool, ghost counter_in:nat) returns (e:Interview<T>, ghost counter_out:nat)
+    requires Valid()
+    requires Model() != Null
+    ensures Valid()
+    ensures e.Model() == if b then Model().True else Model().False
+    ensures e.Questions() == Questions() - {Model().Key}
+    ensures e.Candidates() == (set cand:candidate | cand in Candidates() && cand[Model().Key] == b :: cand)
+    ensures counter_out == counter_in + UBSize()
+  
+
+  method {:axiom} Empty(ghost counter_in:nat) returns (b:bool, ghost counter_out:nat)
+    requires Valid()
+    ensures b == (Model() == Null)
+    ensures counter_out == counter_in + 1
+
+}
