Reduction/ReductionSetCoverToCDPC.dfy
@@ -3,11 +3,12 @@ include "../Problems/SetCover.dfy"
 include "../Auxiliary/Lemmas.dfy"
 
 
-ghost function SetCoverToCDPC(U:set<int>, S:set<set<int>>, k:nat) : (r:(map<Candidate, bool>, map<Candidate, int>, set<int>, real, real, real, real))
+ghost function SetCoverToCDPC(U:set<int>, S:set<set<int>>, k:nat) : (r:(map<candidate, bool>, map<candidate, int>, set<int>, real, real, real, real))
   requires forall s | s in S :: s <= U
   requires isCover(U, S)
+  ensures forall c1, c2:candidate |  c1 in r.0.Keys && c2 in r.0.Keys :: c1.Keys == c2.Keys
   ensures r.0.Keys == r.1.Keys
-  ensures forall c:Candidate | c in r.0.Keys :: (r.2 <= c.Keys)
+  ensures forall c:candidate | c in r.0.Keys :: (r.2 <= c.Keys)
   ensures 0.0 <= r.3 <= r.4 <= 1.0
   ensures 0.0 <= r.5 <= r.6 <= 1.0
 
